Strata/DL/Lambda/LExpr.Test.lean
@@ -38,6 +38,8 @@ def progMotivating: LExpr LTy String :=
     (c.vAt "i" "o"))) <|
   skip
 
+
+
 /--
 info: (declare-const i@0 Int)
 (declare-const b@1 Bool)
